#Section A
##1
###a.

Big Endian: The least significant bit comes last.

| 0 | 1 | 2 | 3 | 4 | 5 | 6 |
|---|---|---|---|---|---|---|
| T | E | S | T | I | N | G |


Little Endian: The least significant bit comes first.

| 0 | 1 | 2 | 3 | 4 | 5 | 6 |
|---|---|---|---|---|---|---|
| G | N | I | T | S | E | T |

###b.

2's Complement (N-bits; N = 4):

| Bit Pattern    | 0000 | ... | 0111            | 1000          | ... | 1111 |
|----------------|------|-----|-----------------|---------------|-----|------|
| 2's Complement | +0   | ... | +2^(N-1)-1 = +7 | -2^(N-1) = -8 | ... | -1   |

-5 = 1011

###c.

Convert -139.325 to binary and hexadecimal using IEEE Single Precision Format (use rounding over truncation).

Without a calculator, I'm not sure how I would do this without rounding to -139.3125 so that's what I'm going to do.

-139.325 in binary is 1000 1011.0101 0011 0011 0011 (truncating)

-139.3125 in binary is 1000 1011.0101 0000 0000 0000 (rounding)

This becomes 1.0001 0110 1010 0000 0000 000 x 2^7

Sign: 1 (negative)

Exponent: 7 + 127 = 134 --binary--> 1000 0110

Significand: 0001 0110 1010 0000 0000 000

Solution = Sign + Exponent + Significand

1100 0011 0000 1011 0101 0000 0000 0000

Binary | 1100 | 0011 | 0000 | 1011 | 0101 | 0000 | 0000 | 0000
-------|------|------|------|------|------|------|------|-----
Hex    | C    | 3    |  0   |  B   |   5  |  0   |  0   | 0


###d.

Equation | Rule
------------ | -------------
E = A' \* (A + B) + (B + A \* A) \* (A + B') | given
E = (A' \* A) + (A' \* B) + (B + A \* A) \* (A + B') | distributive
E = 0 + (A' \* B) + (B + A \* A) \* (A + B') | negation
E = (A' \* B) + (B + A \* A) \* (A + B') | simplification
E = (A' \* B) + (B + A) \* (A + B') | idempotent
E = ((A' \* B) + B) + A \* (A + B') | associative
E = (A' + B) \* (B + B) + A \* (A + B') | distributive
E = (A' + B) \* B + A \* (A + B') | simplification (A + A = A)
E = (A' + 1) \* B + A \* (1 + B') | simplification (A \* 1 = A)
E = 1 \* B + A \* 1 | simplification (A + 1 = 1)
E = A + B | simplification (A \* 1 = A)
