#Section A
### 1a

((p → q) ^ (r → s) ^ (p v r )) → (q v s)

i)

```
((¬p v q) ^ (¬r v s) ^ (p v r )) → (q v s) 

(¬(¬p v q) v ¬(¬r v s) v ¬(p v r)) → (q v s)

(p v q v r v s v ¬p v ¬r) → (q v s)

(p v ¬p r v ¬r v q v s)  → (q v s)

(T v T v q v s) → (q v s)

(q v s) → (q v s)

```

ii)

```
1.  ((p → q) ^ (r → s) ^ (p v r )) assume 
2.  p → q                           1. ^E
3.  r → s
4.  p v r 
5.  ¬(q v s)                       assume
6.  ¬ q ^ ¬ s                      lemma 1
7.  ¬ q 
8.  ¬ s
9.  ¬ p 
10. ¬ r
11. ¬ p ^ ¬ r 
12. ¬ (p v r )                     lemma 2
13. q v s                          RAA 5, 12, 4

lemma 1
¬(q v s) → ¬ q ^ ¬ s 

1. ¬(q v s) assume 
2. q        assume
3. q v s    v I 
4. ¬ q      RAA 1,3

lemma 2 
¬ q ^ ¬ s →  ¬(q v s)

1. ¬ q ^ ¬ s   assume 
2. q v s       assume 
3. ¬ q         ^ E
4. s           v E, 3 
5. ¬ s         ^ E, 1
6, ¬( q v s)   RAA, 2,4,5
```

### 1b

i) 

∀ X (p(X) →  q(X)) implies ∀ X p(X) →  q ∀ X (X)  

```
∀ X (p(X) →  q(X)) 
1. p(a)                        assume
2. q(a)                        → I, 1
3. ∀ X p(X)                    ∀ I
4. ∀ X q(X)                    ∀ I
5. ∀ X p(X) →  ∀ X q(X)        I→  3,4
```

ii)

∃ X (p(X) ^ q(X)) implies ∃ X p(X) ^ ∃ X q(X)

```
∃ X (p(X) ^ q(X))      
1. p(a)                       assume
2. q(a)                       ^ I, 1
3. ∃ X p(X)                   ∃ I,1
4. ∃ X q(X)                   ∃ I,2
5. ∃ X p(X) ^ ∃ X q(X)        ^ I 3,4
```

iii)

∀ X (p(X) →  (∃ Y q(X,Y) →  r(X))). implies  ∀ X (p(X) ^ ¬ r(X) →   ∀ Y
¬q(X,Y)).

```
∀ X (p(X) →  (∃ Y q(X,Y) →  r(X))).

1. p(a)                 assume 
2. q(a,

